@prefix rdf: <http://www.w3.org/1999/02/22-rdf-syntax-ns#> .
@prefix rdfs: <http://www.w3.org/2000/01/rdf-schema#> .
@prefix lite: <http://bibfra.me/vocab/lite/> .
@prefix scholar: <http://bibfra.me/vocab/scholar/> .
@prefix rel: <http://bibfra.me/vocab/relation/> .
@prefix library: <http://bibfra.me/vocab/marc/> .
@prefix link: <http://library.link/identifier/> .
@prefix dc: <http://purl.org/dc/terms/> .
@prefix schema: <http://schema.org/> .
@prefix owl: <http://www.w3.org/2002/07/owl#> .
@prefix bf: <http://id.loc.gov/ontologies/bibframe/> .
@prefix skos: <http://www.w3.org/2004/02/skos/core#> .
@prefix oa: <http://www.w3.org/ns/oa#> .
@prefix foaf: <http://xmlns.com/foaf/0.1/> .
@prefix xsd: <http://www.w3.org/2001/XMLSchema#> .

# BUILDE Scholar Extension üìñüîç
#
# This RDF vocabulary encompasses a wide range of classes and properties suitable for describing various
# types of bibliographic resources, scholarly works, and related entities.
#
# This vocabulary is ideal for librarians, information scientists, data curators, and developers working
# in academic and research settings. It can be employed in creating digital libraries, scholarly databases,
# cataloging systems, and other applications requiring structured bibliographic information.
#
# Key Features:
# - Compatibility with existing ontologies including Schema.org, SKOS, FOAF, and Dublin Core for enhanced interoperability.
# - Extension of BIBFRAME from the Library of Congress
# - Comprehensive coverage of bibliographic and scholarly domains.
# - Clear, self-explanatory labels and definitions for each class and property.
# - Hierarchical organization of classes using rdfs:subClassOf for structured representation.
#
# We encourage users to provide feedback and suggestions to continually improve and update this vocabulary.
# For versioning, updates, and more detailed documentation, please visit [https://bibfra.me/?].
#
scholar: a rdfs:Vocabulary ;
    rdfs:label "Builde Scholar" ;
    rdfs:comment "Builde vocabulary for scholarly research" ;
    dc:creator "EBSCO Information Systems" ;
    dc:created "2024-07-22"^^xsd:date ;
    dc:issued "2024-08-22"^^xsd:date ;
    dc:modified "2024-08-22"^^xsd:date ;
    owl:versionInfo "1.0" .

## BF Scholar Classes (from Crossref)

scholar:Journal a rdfs:Class ;
    rdfs:label "Journal"@en ;
    rdfs:comment "A publication that issues periodic releases containing multiple scholarly articles."@en ;
    owl:sameAs schema:Periodical ;
    rdfs:subClassOf lite:Work .

scholar:Article a rdfs:Class ;
    rdfs:label "Article"@en ;
    rdfs:comment "A written composition on a specific topic, typically published in a journal or magazine."@en ;
    owl:sameAs schema:ScholarlyArticle ;
    rdfs:subClassOf lite:Work .

scholar:BlogEntry a rdfs:Class ;
    rdfs:label "Blog Entry"@en ;
    rdfs:comment "An individual post or entry in a blog, often informal or conversational in style."@en ;
    owl:sameAs schema:Blog ;
    rdfs:subClassOf lite:Work .

scholar:ConferencePaper a rdfs:Class ;
    rdfs:label "Conference Paper"@en ;
    rdfs:comment "A paper presented at a conference and often subsequently published in conference proceedings."@en ;
    owl:sameAs schema:Blog ;
    rdfs:subClassOf scholar:Article .

scholar:ConferenceProceeding a rdfs:Class ;
    rdfs:label "Conference Proceeding"@en ;
    rdfs:comment "A collection of academic papers presented at a professional association meeting or conference."@en ;
    rdfs:subClassOf lite:Work .

scholar:Database a rdfs:Class ;
    rdfs:label "Database"@en ;
    rdfs:comment "An organized collection of data or information, often electronic."@en ;
    rdfs:subClassOf lite:Work .

scholar:Dataset a rdfs:Class ;
    rdfs:label "Dataset"@en ;
    rdfs:comment "A body of structured information describing some topic(s) of interest."@en ;
    owl:sameAs schema:Dataset ;
    rdfs:subClassOf lite:Work .

scholar:Dissertation a rdfs:Class ;
    rdfs:label "Dissertation"@en ;
    rdfs:comment "Formal document presenting original research conducted by a candidate for a doctoral degree, demonstrating the candidate's expertise and contribution to their field of study."@en ;
    owl:sameAs schema:Thesis ;
    rdfs:subClassOf lite:Work .

scholar:Libguide a rdfs:Class ;
	rdfs:label "Libguide"@en ;
	rdfs:comment "Online research guide created by librarians to provide curated resources, information, and instructional content on a specific subject or topic to assist library users."@en ;
	rdfs:subClassOf lite:Work .

scholar:GovernmentDocument a rdfs:Class ;
    rdfs:label "Government Document"@en ;
    rdfs:comment "An official publication issued by a government or international body."@en ;
    rdfs:subClassOf scholar:Report .

scholar:Newspaper a rdfs:Class ;
    rdfs:label "Newspaper"@en ;
    rdfs:comment "A publication containing news, articles, advertisements, and other content, usually issued daily or weekly."@en ;
    owl:sameAs schema:Newspaper ;
    rdfs:subClassOf lite:Work .

scholar:Periodical a rdfs:Class ;
    rdfs:label "Periodical"@en ;
    rdfs:comment "A publication released at regular intervals, such as journals, magazines, or newspapers."@en ;
    owl:sameAs schema:Periodical ;
    rdfs:subClassOf lite:Work .

scholar:PrimarySourceDocument a rdfs:Class ;
    rdfs:label "Primary Source Document"@en ;
    rdfs:comment "An original document or firsthand account relevant to historical or research study."@en ;
    rdfs:subClassOf lite:Work .

scholar:Report a rdfs:Class ;
    rdfs:label "Report"@en ;
    rdfs:comment "A formal account or statement describing the findings of some individual or group."@en ;
    owl:sameAs schema:Report ;
    rdfs:subClassOf lite:Work .

scholar:Review a rdfs:Class ;
    rdfs:label "Review"@en ;
    rdfs:comment "A critical assessment or analysis of a subject or work, especially in the form of an article."@en ;
    rdfs:subClassOf scholar:Article .

scholar:TradePublication a rdfs:Class ;
    rdfs:label "Trade Publication"@en ;
    rdfs:comment "A periodical publication targeted towards professionals in a specific industry."@en ;
    rdfs:subClassOf scholar:Periodical .

scholar:Wires a rdfs:Class ;
    rdfs:label "WIRES"@en ;
    rdfs:comment "A work within the Wiley Interdisciplinary Reviews series, characterized as a peer-reviewed, expert-authored review article that spans multiple interdisciplinary fields. This work is tailored to various audiences, including students, interdisciplinary collaborators, and experts, offering comprehensive overviews, specific technological insights, and up-to-date knowledge in respective fields."@en ;
    rdfs:subClassOf lite:Work .

scholar:WorkingPaper a rdfs:Class ;
    rdfs:label "Working Paper"@en ;
    rdfs:comment "A preliminary scientific or technical paper often published to share ideas about a topic before formal publication."@en ;
    rdfs:subClassOf scholar:Article .

scholar:Award a rdfs:Class ;
    rdfs:label "Award"@en ;
    rdfs:comment "A recognition or honor awarded typically for academic, artistic, or scientific achievement."@en ;
    rdfs:subClassOf lite:Resource .

scholar:SubAward a rdfs:Class ;
    rdfs:label "Subaward"@en ;
    rdfs:comment "A subaward is a financial or contractual agreement made by the primary recipient (or \"prime\") of a grant, contract, or cooperative agreement to a secondary recipient, referred to as a subrecipient or subawardee."@en ;
    rdfs:subClassOf scholar:Award .

scholar:Grant a rdfs:Class ;
    rdfs:label "Grant"@en ;
    rdfs:comment "A grant is a sum of money given by an organization, especially a government, to a person or entity for a specific purpose that does not require repayment."@en ;
    rdfs:subClassOf lite:Resource .

scholar:CooperativeAgreement a rdfs:Class ;
    rdfs:label "Grant"@en ;
    rdfs:comment "A cooperative agreement is a form of financial assistance provided by a federal agency to a recipient to carry out a public purpose of support or stimulation, where substantial involvement is expected between the agency and the recipient during the performance of the contemplated activity."@en ;
    rdfs:subClassOf lite:Resource .

scholar:DirectPayment a rdfs:Class ;
    rdfs:label "Direct Payment"@en ;
    rdfs:comment "A direct payment is a transfer of funds from one party directly to another without the need for intermediaries, typically made electronically for the purpose of settling debts, transactions, or fulfilling financial obligations."@en ;
    rdfs:subClassOf lite:Resource .

scholar:Loan a rdfs:Class ;
    rdfs:label "Loan"@en ;
    rdfs:comment "A loan is a sum of money borrowed by one party from another, which must be repaid with interest over a defined period."@en ;
    rdfs:subClassOf lite:Resource .

scholar:Insurance a rdfs:Class ;
    rdfs:label "Insurance"@en ;
    rdfs:comment "Insurance is a contract represented by a policy, in which an individual or entity receives financial protection or reimbursement against losses from an insurance company."@en ;
    rdfs:subClassOf lite:Resource .

scholar:FundingAward a rdfs:Class ;
    rdfs:label "Funding Award"@en ;
    rdfs:comment "Financial support provided for research or a scholarly project."@en ;
    rdfs:subClassOf scholar:Award .

scholar:Agency a rdfs:Class ;
    rdfs:label "Agency"@en ;
    rdfs:comment "An administrative unit or organization, often governmental, with a specific purpose or function."@en ;
    rdfs:subClassOf lite:Organization .

scholar:Program a rdfs:Class ;
    rdfs:label "Program"@en ;
    rdfs:comment "A program refers to a structured set of activities designed to achieve specific outcomes or objectives, often related to research, education, or community service."@en ;
    rdfs:subClassOf lite:Resource .

scholar:Nonprofit a rdfs:Class ;
    rdfs:label "Nonprofit"@en ;
    rdfs:comment "An organization dedicated to furthering a particular social cause or advocating for a shared point of view, not for profit."@en ;
    rdfs:subClassOf lite:Organization .
	
scholar:Facility a rdfs:Class ;
    rdfs:label "Facility"@en ;
    rdfs:comment "A place, amenity, or piece of equipment provided for a particular purpose within the scholarly context, such as research laboratories or lecture halls."@en ;
    rdfs:subClassOf lite:Place .

scholar:Company a rdfs:Class ;
    rdfs:label "Company"@en ;
    rdfs:comment "A legal entity formed by a group of individuals to engage in and operate a business‚Äîcommercial or industrial‚Äîenterprise."@en ;
    rdfs:subClassOf lite:Organization .

scholar:Healthcare a rdfs:Class ;
    rdfs:label "Healthcare Organization"@en ;
    rdfs:comment "A field involved in the maintenance or improvement of health via the prevention, diagnosis, treatment, recovery, or cure of disease, illness, injury, and other physical and mental impairments in people."@en ;
    rdfs:subClassOf lite:Organization .

scholar:University a rdfs:Class ;
    rdfs:label "University"@en ;
    rdfs:comment "An institution of higher learning providing facilities for teaching and research and authorized to grant academic degrees."@en ;
    rdfs:subClassOf lite:Organization .

scholar:Consortia a rdfs:Class ;
    rdfs:label "Consortia"@en ;
    rdfs:comment "An association or combination of businesses, financial institutions, universities, or other organizations who pool resources and expertise to achieve a common goal."@en ;
    rdfs:subClassOf lite:Organization .

scholar:Faculty a rdfs:Class ;
    rdfs:label "Faculty"@en ;
    rdfs:comment "academic staff of a university or college, including professors, lecturers, and researchers, who are responsible for teaching and conducting research."@en ;
    rdfs:subClassOf lite:Person .

scholar:School a rdfs:Class ;
    rdfs:label "School"@en ;
    rdfs:comment "An institution for educating children or a department or faculty of a college concerned with a particular subject."@en ;
    rdfs:subClassOf lite:Organization .

scholar:Department a rdfs:Class ;
    rdfs:label "Department"@en ;
    rdfs:comment "A division of a larger organization such as a university, dealing with a specific subject of study or research."@en ;
    rdfs:subClassOf lite:Organization .
	
scholar:College a rdfs:Class ;
    rdfs:label "College"@en ;
    rdfs:comment "An educational institution or a constituent part of one that awards degrees in various academic disciplines."@en ;
    rdfs:subClassOf lite:Organization .

scholar:ror a rdf:Property ;
    rdfs:label "research organization registry ID"@en ;
    rdfs:comment "An organization's Research Organization Registry open persistent identifier."@en ;
    rdfs:domain scholar:Organization ;
    rdfs:range rdfs:Literal  .

scholar:BookReview a rdfs:Class ;
    rdfs:label "Book Review"@en ;
    rdfs:comment "A book review is a critical evaluation of a book, often published in a periodical, that discusses its content, style, and merit."@en ;
    rdfs:subClassOf lite:Work .

scholar:Chapter a rdfs:Class ;
    rdfs:label "Chapter"@en ;
    rdfs:comment "A main division of a book, typically with a number or title."@en ;
    rdfs:subClassOf lite:Work .
	
scholar:Part a rdfs:Class ;
    rdfs:label "Part"@en ;
    rdfs:comment "A division within a book or publication that may contain chapters or other sections."@en ;
    rdfs:subClassOf lite:Work .

scholar:Repository a rdfs:Class ;
    rdfs:label "Repository"@en ;
    rdfs:comment "A central location in which data is stored and managed, often used in the context of academic and scholarly research for the storage of datasets, publications, and digital archives."@en ;
    rdfs:subClassOf lite:Resource .
	
scholar:Magazine a rdfs:Class ;
    rdfs:label "Magazine"@en ;
    rdfs:comment "A periodical publication containing articles and illustrations, typically covering a particular subject or area of interest."@en ;
    rdfs:subClassOf lite:Resource .
	
scholar:Trade a rdfs:Class ;
    rdfs:label "Trade"@en ;
    rdfs:comment "A trade publication is a magazine or journal dedicated to topics relevant to a specific industry or professional field, aimed at professionals within that field."@en ;
    rdfs:subClassOf lite:Work .

scholar:Artifact a rdfs:Class ;
    rdfs:label "Artifact"@en ;
    rdfs:comment "An object made by a human being, typically an item of cultural or historical interest."@en ;
    rdfs:subClassOf lite:Work .

scholar:Thesis a rdfs:Class ;
    rdfs:label "Thesis"@en ;
    rdfs:comment "A document submitted in support of candidature for an academic degree or professional qualification presenting the author's research and findings."@en ;
    rdfs:subClassOf scholar:Report .

scholar:Abstract a rdfs:Class ;
    rdfs:label "Abstract"@en ;
    rdfs:comment "A brief summary of a research article, thesis, review, conference proceeding, or any in-depth analysis of a particular subject or discipline."@en ;
    rdfs:subClassOf lite:Work .

scholar:AnnualReport a rdfs:Class ;
    rdfs:label "Annual Report"@en ;
    rdfs:comment "A comprehensive report on a company's activities throughout the preceding year."@en ;
    rdfs:subClassOf scholar:Report .

scholar:Citation a rdfs:Class ;
    rdfs:label "Citation"@en ;
    rdfs:comment "A reference to a book, paper, or author, especially in scholarly work."@en ;
    rdfs:subClassOf lite:Resource .

scholar:CurriculumVitae a rdfs:Class ;
    rdfs:label "Curriculum Vitae"@en ;
    rdfs:comment "A written overview of a person's experience and other qualifications for a job opportunity."@en ;
    rdfs:subClassOf lite:Resource .

scholar:Editorial a rdfs:Class ;
    rdfs:label "Editorial"@en ;
    rdfs:comment "An article written by the editor or senior staff of a publication expressing an opinion on a topical issue."@en ;
    rdfs:subClassOf scholar:Article .

scholar:Exhibition a rdfs:Class ;
    rdfs:label "Exhibition"@en ;
    rdfs:comment "A public display of works of art or items of interest, held in an art gallery or museum or at a trade fair."@en ;
    rdfs:subClassOf lite:Work .

scholar:ExtensionPublication a rdfs:Class ;
    rdfs:label "Extension Publication"@en ;
    rdfs:comment "A publication intended to provide university research findings and education to the community, often through cooperative extension services."@en ;
    rdfs:subClassOf scholar:Report .

scholar:Handbook a rdfs:Class ;
    rdfs:label "Handbook"@en ;
    rdfs:comment "A book giving information such as facts on a particular subject or instructions for operating a machine or system."@en ;
    rdfs:subClassOf lite:Work .

scholar:InstructionalPlan a rdfs:Class ;
    rdfs:label "Instructional Plan"@en ;
    rdfs:comment "A detailed description designed to teach a particular subject or activity."@en ;
    rdfs:subClassOf lite:Resource .

scholar:LearningObject a rdfs:Class ;
    rdfs:label "Learning Object"@en ;
    rdfs:comment "A resource, usually digital and online, used to support learning objectives."@en ;
    rdfs:subClassOf lite:Resource .

scholar:MajorPaper a rdfs:Class ;
    rdfs:label "Major Paper"@en ;
    rdfs:comment "A significant academic paper written as part of a graduate program, reflecting the outcome of research or study."@en ;
    rdfs:subClassOf scholar:Report .

scholar:MastersProject a rdfs:Class ;
    rdfs:label "Masters Project"@en ;
    rdfs:comment "A comprehensive project undertaken as part of the requirement for a master's degree."@en ;
    rdfs:subClassOf scholar:Report .

scholar:Patent a rdfs:Class ;
    rdfs:label "Patent"@en ;
    rdfs:comment "A government authority or license conferring a right or title for a set period, especially the sole right to exclude others from making, using, or selling an invention."@en ;
    rdfs:subClassOf lite:Work .

scholar:Poster a rdfs:Class ;
    rdfs:label "Poster"@en ;
    rdfs:comment "A large printed picture, photograph, or notice used to advertise something or as a decoration."@en ;
    rdfs:subClassOf lite:Work .

scholar:Presentation a rdfs:Class ;
    rdfs:label "Presentation"@en ;
    rdfs:comment "A talk or speech given to a live or virtual audience about a particular topic."@en ;
    rdfs:subClassOf lite:Work .

scholar:PressRelease a rdfs:Class ;
    rdfs:label "Press Release"@en ;
    rdfs:comment "An official statement issued to newspapers and other news media for the purpose of providing information, an official announcement, or making a public statement."@en ;
    rdfs:subClassOf lite:Work .

scholar:Proposal a rdfs:Class ;
    rdfs:label "Proposal"@en ;
    rdfs:comment "A plan or suggestion, especially a formal or written one, put forward for consideration by others."@en ;
    rdfs:subClassOf lite:Work .

scholar:Software a rdfs:Class ;
    rdfs:label "Software"@en ;
    rdfs:comment "A program or set of programs that instruct a computer to perform specific tasks."@en ;
    rdfs:subClassOf lite:Work .

scholar:SpecialReport a rdfs:Class ;
    rdfs:label "Special Report"@en ;
    rdfs:comment "A detailed and comprehensive analysis on a specific topic or event."@en ;
    rdfs:subClassOf scholar:Report .

scholar:Summary a rdfs:Class ;
    rdfs:label "Summary"@en ;
    rdfs:comment "A brief statement or account covering the main points of a larger work or article."@en ;
    rdfs:subClassOf lite:Work .

scholar:SlideShow a rdfs:Class ;
    rdfs:label "Slide Show"@en ;
    rdfs:comment "A presentation of a series of still images on a projection screen or electronic display device, typically in a prearranged sequence."@en ;
    rdfs:subClassOf lite:Work .

scholar:Publisher a rdfs:Class ;
    rdfs:label "Publisher"@en ;
    rdfs:comment "An entity responsible for making the resource available, including companies, organizations, or individuals."@en ;
    rdfs:subClassOf lite:ProviderAgent .

scholar:Policy a rdfs:Class ;
    rdfs:label "Policy"@en ;
    rdfs:comment "A course or principle of action adopted or proposed by an organization or individual."@en ;
    rdfs:subClassOf lite:Resource .

scholar:OpenAccessPolicy a rdfs:Class ;
    rdfs:label "Open Access Policy"@en ;
    rdfs:comment "A policy that promotes open access to scholarly works and resources."@en ;
    rdfs:subClassOf scholar:Policy .

scholar:DepositAccess a rdfs:Class ;
    rdfs:label "Deposit Access"@en ;
    rdfs:comment "Policies or guidelines related to the depositing of scholarly works into repositories or archives."@en ;
    rdfs:subClassOf scholar:Policy .

scholar:ActionEvent a rdfs:Class ;
    rdfs:label "Action Event"@en ;
    rdfs:comment "Represents an action or event within the lifecycle of a scholarly activity, such as the awarding of a grant, submission of a paper, or any other significant occurrence that has implications for the research or academic work."@en ;
    rdfs:subClassOf lite:Event .

## Scholar Identifier Classes
	
scholar:DOI a rdfs:Class ;
    rdfs:label "DOI"@en ;
    rdfs:comment "A persistent identifier or handle used to uniquely identify various objects, standardized by the International Organization for Standardization."@en ;
    rdfs:subClassOf lite:Identifier .

scholar:OpenAlexID a rdfs:Class ;
    rdfs:label "Open Alex ID"@en ;
    rdfs:comment "A persistent identifier used to uniquely identify various entities within the OpenAlex dataset, including scholarly works, authors, and institutions."@en ;
    rdfs:subClassOf lite:Identifier .

## Scholar Properties for Person

scholar:orcid a rdf:Property ;
    rdfs:label "ORCID"@en ;
    rdfs:comment "An ORCID persistent digital identifier for a researcher."@en ;
    rdfs:domain lite:Person ;
    rdfs:range link:ORCID  .

scholar:affiliation a rdf:Property ;
    rdfs:label "affiliation"@en ;
    rdfs:comment "The affiliated institution or organization of a person."@en ;
    rdfs:domain lite:Person ;
    rdfs:range lite:Organization .

scholar:suffix a rdf:Property ;
    rdfs:label "suffix"@en ;
    rdfs:comment "A suffix indicating academic or professional status, e.g., PhD, MD."@en ;
    rdfs:domain lite:Person ;
    rdfs:range rdfs:Literal  .

scholar:interest a rdf:Property ;
    rdfs:label "interest"@en ;
    rdfs:comment "Specifies the interest or research area of an individual or entity in the context of scholarly work."@en ;
    rdfs:range lite:Concept ;
    rdfs:domain lite:Person .

scholar:discipline a rdf:Property ;
    rdfs:label "discipline"@en ;
    rdfs:comment "A field of study or academic discipline related to a person."@en ;
    rdfs:range lite:Concept ;
    rdfs:domain lite:Person .

scholar:mostCitedWork a rdf:Property ;
    rdfs:label "most cited work"@en ;
    rdfs:comment "Title of the most cited work by a person."@en ;
    rdfs:range lite:Work ;
    rdfs:domain lite:Person .

## ID properties

scholar:fainId a rdf:Property ;
    rdfs:label "fain ID"@en ;
    rdfs:comment "A unique identifier for a funding award."@en ;
    rdfs:domain scholar:FundingAward ;
    rdfs:range rdfs:Literal .

scholar:openalexId a rdf:Property ;
    rdfs:label "openalex ID"@en ;
    rdfs:comment "A unique identifier used in the OpenAlex database to reference various scholarly entities, such as works, authors, institutions, publishers, and topics."@en ;
    rdfs:domain lite:Resource ;
    rdfs:range rdfs:Literal .
	
scholar:doi a rdf:Property ;

    rdfs:label "doi"@en ;
    rdfs:comment "A persistent identifier or handle used to uniquely identify various objects, standardized by the International Organization for Standardization."@en ;
    rdfs:domain scholar:Article ;
    rdfs:range rdfs:Literal ;
    rdfs:range rdfs:Literal .
	
## Crossref property for Award

scholar:award a rdf:Property ;
    rdfs:label "award"@en ;
    rdfs:comment "An award associated with a person, organization, or resource."@en ;
    owl:equivalentProperty schema:award ;
    rdfs:domain lite:Agent ;
    rdfs:range scholar:Award .

## Scholar properties for Work, Article, Award, and Journal

scholar:cites a rdf:Property ;
    rdfs:label "cites"@en ;
    rdfs:comment "Links the citing work to the cited work."@en ;
    rdfs:domain lite:Work ;
    rdfs:range lite:Work .

scholar:citedBy a rdf:Property ;
    rdfs:label "citedBy"@en ;
    rdfs:comment "Links cited work to the citing work."@en ;
    rdfs:domain lite:Work ;
    rdfs:range lite:Work .

scholar:citedByCount a rdf:Property ;
    rdfs:label "cited by count"@en ;
    rdfs:comment "The number of times a Work has been cited."@en ;
    rdfs:range rdfs:Literal ;
    rdfs:domain lite:Resource .

scholar:worksCount a rdf:Property ;
    rdfs:label "works count"@en ;
    rdfs:comment "The number of works associated with a resource."@en ;
    rdfs:range rdfs:Literal ;
    rdfs:domain lite:Resource .

scholar:countsByYear a rdf:Property ;
    rdfs:label "counts by year"@en ;
    rdfs:comment "The number of works associated with a resource organized by year."@en ;
    rdfs:range rdfs:Literal ;
    rdfs:domain lite:Resource .

scholar:citationCount a rdf:Property ;
    rdfs:label "citation count"@en ;
    rdfs:comment "The number of citations used by a Work."@en ;
    rdfs:range rdfs:Literal ;
    rdfs:domain lite:Work .

scholar:articleVersion a rdf:Property ;
    rdfs:label "article version"@en ;
    rdfs:comment "Specifies the version of the article in context, such as preprint, postprint, or published version."@en ;
    rdfs:range rdfs:Literal ;
    rdfs:domain scholar:Article .

scholar:articleLocation a rdf:Property ;
    rdfs:label "article location"@en ;
    rdfs:comment "Location where the article can be accessed, such as a URL or physical location in a library."@en ;
    rdfs:range lite:link ;
    rdfs:domain scholar:Article .

scholar:xLink a rdf:Property ;
    rdfs:label "X link"@en ;
    rdfs:comment "Link that directs users to a specific page or content on the social media platform X, which was previously known as Twitter."@en ;
    rdfs:range lite:link ;
    rdfs:domain scholar:Article .

scholar:action a rdf:Property ;
    rdfs:label "action"@en ;
    rdfs:comment "An action taken in the context of an award, such as granting, renewing, or revising."@en ;
    rdfs:range lite:Resource ;
    rdfs:domain scholar:Award .

scholar:actionOf a rdf:Property ;
    rdfs:label "action of"@en ;
    rdfs:comment "The award or program to which an action pertains."@en ;
    rdfs:range [
        a owl:Class ;
        owl:unionOf (scholar:Award scholar:Program)
    ] ;
    rdfs:domain scholar:ActionEvent .

scholar:fundedBy a rdf:Property ;
    rdfs:label "funded by"@en ;
    rdfs:comment "Specifies the entity that provides funding for an award or project."@en ;
    rdfs:range lite:Agent ;
    rdfs:domain scholar:Award .

scholar:awardedBy a rdf:Property ;
    rdfs:label "awarded by"@en ;
    rdfs:comment "The entity responsible for awarding a grant, fellowship, or honor."@en ;
    rdfs:range lite:Agent ;
    rdfs:domain scholar:Award .

scholar:awardRecipient a rdf:Property ;
    rdfs:label "award recipient"@en ;
    rdfs:comment "The individual or organization that receives an award or grant."@en ;
    rdfs:subPropertyOf rel:recipient ;
    rdfs:range lite:Agent ;
    rdfs:domain scholar:Award .

scholar:awardedTo a rdf:Property ;
    rdfs:label "awarded to"@en ;
    rdfs:comment "Indicates the recipient of an award."@en ;
    rdfs:range lite:Agent ;
    rdfs:domain scholar:Award .

scholar:isSubAwardOf a rdf:Property ;
    rdfs:label "is sub award of"@en ;
    rdfs:comment "Indicates that an award is a sub-award of a larger grant or funding mechanism."@en ;
    rdfs:range scholar:Award ;
    rdfs:domain scholar:SubAward .

scholar:coAwardedTo a rdf:Property ;
    rdfs:label "co-awarded to"@en ;
    rdfs:comment "Indicates additional recipients who are co-awarded a grant or honor."@en ;
    rdfs:range lite:Agent ;
    rdfs:domain scholar:Award .
	
scholar:supportedBy a rdf:Property ;
    rdfs:label "supported by"@en ;
    rdfs:comment "Identifies the supporting entity or funding source for a project, publication, or award."@en ;
    rdfs:range lite:Agent ;
    rdfs:domain scholar:Award .

scholar:isRetracted a rdf:Property ;
    rdfs:label "is retracted"@en ;
    rdfs:comment "Indicates whether an article has been officially withdrawn from publication due to issues such as errors or ethical concerns."@en ;
    rdfs:range xsd:boolean ;
    rdfs:domain scholar:Article .

scholar:firstAuthor a rdf:Property ;
    rdfs:label "first author"@en ;
    rdfs:comment "Identifies the primary or lead author of an article, typically listed first among the authors."@en ;
    rdfs:range lite:Person ;
    rdfs:domain scholar:Article .

scholar:middleAuthor a rdf:Property ;
    rdfs:label "middle author"@en ;
    rdfs:comment "Identifies an author listed between the first and last author in a multi-authored article, often contributing significantly to the research."@en ;
    rdfs:range lite:Person ;
    rdfs:domain scholar:Article .

scholar:lastAuthor a rdf:Property ;
    rdfs:label "last author"@en ;
    rdfs:comment "Identifies the author listed last in a multi-authored article, often signifying a senior or supervising role in the research."@en ;
    rdfs:range lite:Person ;
    rdfs:domain scholar:Article .

scholar:publishedIn a rdf:Property ;
    rdfs:label "published in"@en ;
    rdfs:comment "Relates an article or paper to the journal where it was published."@en ;
    rdfs:range lite:Article ;
    rdfs:subPropertyOf rel:isPartOf ;
    rdfs:domain scholar:Journal .

### Publisher Policy Edges

scholar:providerPolicy a rdf:Property ;
    rdfs:label "provider policy"@en ;
    rdfs:comment "A policy specified by the provider or publisher regarding the dissemination or usage of the content."@en ;
    rdfs:range lite:Policy ;
    rdfs:domain lite:Instance .

scholar:providerDepositLocation a rdf:Property ;
    rdfs:label "provider deposit location"@en ;
    rdfs:comment "The location where the provider deposits the scholarly content, such as an institutional or subject repository."@en ;
    rdfs:range lite:Repository ;
    rdfs:domain lite:Instance .

scholar:copyrightOwner a rdf:Property ;
    rdfs:label "copyright owner"@en ;
    rdfs:comment "The entity that holds the copyright of the scholarly content."@en ;
    rdfs:range lite:Agent ;
    rdfs:domain lite:Instance .

scholar:issue a rdf:Property ;
    rdfs:label "issue"@en ;
    rdfs:comment "Specific issue of a journal within a series of published volumes."@en ;
    rdfs:domain lite:Journal ;
    rdfs:range rdfs:Literal .

scholar:volume a rdf:Property ;
    rdfs:label "volume"@en ;
    rdfs:comment "Specific volume of a journal in which a set of issues is published."@en ;
    rdfs:domain lite:Journal ;
    rdfs:range rdfs:Literal .

### Scholar Agency and Program properties

scholar:fundingAgency a rdf:Property ;
    rdfs:label "funding agency"@en ;
    rdfs:comment "The agency or organization that provides funding for the research or project."@en ;
    rdfs:range lite:Agent ;
    rdfs:domain lite:Work .

scholar:awardingAgency a rdf:Property ;
    rdfs:label "awarding agency"@en ;
    rdfs:comment "The agency or organization that awards a grant, prize, or recognition."@en ;
    rdfs:range lite:Agent ;
    rdfs:domain lite:Work .

scholar:programOf a rdf:Property ;
    rdfs:label "program of"@en ;
    rdfs:comment "Associates a project or research with a larger program or initiative."@en ;
    rdfs:range lite:Program ;
    rdfs:domain lite:Work .

scholar:officer a rdf:Property ;
    rdfs:label "officer"@en ;
    rdfs:comment "A person holding an official position in an organization, typically related to oversight or management of a program or project."@en ;
    rdfs:range lite:Program ;
    rdfs:domain lite:Work .
